Set up model_E1E2_L2_orutt_strict_sound.

src/coq/Semantics/InfiniteToFinite/LangRefine.v
@@ -2113,6 +2113,100 @@ Module Type LangRefine (IS1 : InterpreterStack) (IS2 : InterpreterStack) (AC1 : 
     }
   Defined.
 
+  Definition L2_refine_strict A B (e1 : IS1.LP.Events.L2 A) (e2 : IS2.LP.Events.L2 B) : Prop.
+  Proof.
+    refine (match e1, e2 with
+            | inl1 (E1.ExternalCall dt1 f1 args1), inl1 (E2.ExternalCall dt2 f2 args2) =>
+                _
+            | inr1 (inl1 (E1.Intrinsic dt1 name1 args1)), inr1 (inl1 (E2.Intrinsic dt2 name2 args2)) =>
+                _ (* IntrinsicE *)
+            | inr1 (inr1 (inl1 e1)), inr1 (inr1 (inl1 e2)) =>
+                _ (* MemoryE *)
+            | inr1 (inr1 (inr1 (inl1 e1))), inr1 (inr1 (inr1 (inl1 e2))) =>
+                _ (* PickE *)
+            | inr1 (inr1 (inr1 (inr1 (inl1 e0)))), inr1 (inr1 (inr1 (inr1 (inl1 e1)))) =>
+                _ (* OOME *)
+            | inr1 (inr1 (inr1 (inr1 (inr1 (inl1 e1))))), inr1 (inr1 (inr1 (inr1 (inr1 (inl1 e2))))) =>
+                _ (* UBE *)
+            | inr1 (inr1 (inr1 (inr1 (inr1 (inr1 (inl1 e1)))))), inr1 (inr1 (inr1 (inr1 (inr1 (inr1 (inl1 e2)))))) =>
+                _ (* DebugE *)
+            | inr1 (inr1 (inr1 (inr1 (inr1 (inr1 (inr1 e1)))))), inr1 (inr1 (inr1 (inr1 (inr1 (inr1 (inr1 e2)))))) =>
+                _ (* FailureE *)
+            | _, _ =>
+                (* Mismatch of event types *)
+                False
+            end).
+
+    (* External Calls *)
+    { (* Doesn't say anything about return value... *)
+      apply (dt1 = dt2 /\
+               uvalue_refine_strict f1 f2 /\
+               Forall2 dvalue_refine_strict args1 args2).
+    }
+
+    (* Intrinsics *)
+    { apply (dt1 = dt2 /\
+               name1 = name2 /\
+               Forall2 dvalue_refine_strict args1 args2).
+    }
+
+    (* MemoryE *)
+    { inversion e1.
+      - (* MemPush *)
+        destruct e2 eqn:HE2.
+        2-5: apply False.
+
+        apply True.
+      - (* MemPop *)
+        destruct e2 eqn:HE2.
+        2: apply True.
+        all: apply False.
+      - (* Alloca *)
+        destruct e2 eqn:HE2.
+        1,2,4,5: apply False.
+
+        apply (t = t0 /\
+                 num_elements = num_elements0 /\
+                 align = align0).
+      - (* Load *)
+        destruct e2 eqn:HE2.
+        1-3,5: apply False.
+        apply (t = t0 /\
+                 dvalue_refine_strict a a0).
+      - (* Store *)
+        destruct e2 eqn:HE2.
+        1-4: apply False.
+
+        apply (t = t0 /\
+                 dvalue_refine_strict a a0 /\
+                 uvalue_refine_strict v v0).
+    }
+
+    (* PickE *)
+    { (* TODO: confirm whether this is sane... *)
+      inversion e1.
+      destruct e2 eqn:HE2.
+      apply ((Pre <-> Pre0) /\
+               uvalue_refine_strict x x0).
+    }
+
+    (* OOME *)
+    { apply True.
+    }
+
+    (* UBE *)
+    { apply True.
+    }
+
+    (* DebugE *)
+    { apply True.
+    }
+
+    (* FailureE *)
+    { apply True.
+    }
+  Defined.
+
   Definition event_converted_lazy A B (e1 : IS1.LP.Events.L0 A) (e2 : IS2.LP.Events.L0 B) : Prop.
   Proof.
     refine (match e1, e2 with
@@ -2632,6 +2726,112 @@ Module Type LangRefine (IS1 : InterpreterStack) (IS2 : InterpreterStack) (AC1 : 
         destruct e2 eqn:HE2.
         + apply False.
         + apply True.
+    }
+
+    (* MemoryE *)
+    { inversion e1; subst.
+      - (* MemPush *)
+        destruct e2 eqn:HE2.
+        2-5: apply False.
+
+        apply True.
+      - (* MemPop *)
+        destruct e2 eqn:HE2.
+        2: apply True.
+        all: apply False.
+      - (* Alloca *)
+        destruct e2 eqn:HE2.
+        1,2,4,5: apply False.
+
+        apply (t = t0 /\
+                 num_elements = num_elements0 /\
+                 align = align0 /\
+                 dvalue_refine_strict res1 res2).
+      - (* Load *)
+        destruct e2 eqn:HE2.
+        1-3,5: apply False.
+        apply (t = t0 /\
+                 dvalue_refine_strict a a0 /\
+                 uvalue_refine_strict res1 res2).
+      - (* Store *)
+        destruct e2 eqn:HE2.
+        1-4: apply False.
+
+        apply (t = t0 /\
+                 dvalue_refine_strict a a0 /\
+                 uvalue_refine_strict v v0).
+    }
+
+    (* PickE *)
+    { (* TODO: confirm whether this is sane... *)
+      inversion e1; subst.
+      destruct e2 eqn:HE2.
+      destruct res1 as [r1 P1].
+      destruct res2 as [r2 P2].
+      apply ((Pre <-> Pre0) /\
+               uvalue_refine_strict x x0 /\
+               dvalue_refine_strict r1 r2).
+    }
+
+    (* OOME *)
+    { apply True.
+    }
+
+    (* UBE *)
+    { apply True.
+    }
+
+    (* DebugE *)
+    { apply True.
+    }
+
+    (* FailureE *)
+    { apply True.
+    }
+  Defined.
+
+  Definition L2_res_refine_strict A B (e1 : IS1.LP.Events.L2 A) (res1 : A) (e2 : IS2.LP.Events.L2 B) (res2 : B) : Prop.
+  Proof.
+    refine (match e1, e2 with
+            | inl1 e1, inl1 e2 =>
+                _
+            | inr1 (inl1 e1), inr1 (inl1 e2) =>
+                _ (* IntrinsicE *)
+            | inr1 (inr1 (inl1 e1)), inr1 (inr1 (inl1 e2)) =>
+                _ (* MemoryE *)
+            | inr1 (inr1 (inr1 (inl1 e1))), inr1 (inr1 (inr1 (inl1 e2))) =>
+                _ (* PickE *)
+            | inr1 (inr1 (inr1 (inr1 (inl1 e0)))), inr1 (inr1 (inr1 (inr1 (inl1 e1)))) =>
+                _ (* OOME *)
+            | inr1 (inr1 (inr1 (inr1 (inr1 (inl1 e1))))), inr1 (inr1 (inr1 (inr1 (inr1 (inl1 e2))))) =>
+                _ (* UBE *)
+            | inr1 (inr1 (inr1 (inr1 (inr1 (inr1 (inl1 e1)))))), inr1 (inr1 (inr1 (inr1 (inr1 (inr1 (inl1 e2)))))) =>
+                _ (* DebugE *)
+            | inr1 (inr1 (inr1 (inr1 (inr1 (inr1 (inr1 e1)))))), inr1 (inr1 (inr1 (inr1 (inr1 (inr1 (inr1 e2)))))) =>
+                _ (* FailureE *)
+            | _, _ =>
+                (* Mismatch of event types *)
+                False
+            end).
+    (* External Calls *)
+    { inv e1.
+      inv e2.
+
+      apply (t = t0 /\
+               uvalue_refine_strict f f0 /\
+               Forall2 dvalue_refine_strict args args0 /\
+               dvalue_refine_strict res1 res2
+            ).
+    }
+
+    (* Intrinsics *)
+    { inv e1.
+      inv e2.
+      apply (t = t0 /\
+               f = f0 /\
+               Forall2 dvalue_refine_strict args args0 /\
+               dvalue_refine_strict res1 res2
+            ).
     }
 
     (* MemoryE *)
@@ -3313,6 +3513,14 @@ Module Type LangRefine (IS1 : InterpreterStack) (IS2 : InterpreterStack) (AC1 : 
       (global_refine_strict × dvalue_refine_strict)
       t1 t2 (OOM:=OOME).
 
+  Definition L2_E1E2_orutt_strict t1 t2
+    : Prop :=
+    orutt
+      L2_refine_strict
+      L2_res_refine_strict
+      (local_refine_strict × stack_refine_strict × (global_refine_strict × dvalue_refine_strict))
+      t1 t2 (OOM:=OOME).
+
   Definition model_E1E2_L0_orutt_strict p1 p2 :=
     L0_E1E2_orutt_strict
       (LLVM1.denote_vellvm (DTYPE_I 32%N) "main" LLVM1.main_args (convert_types (mcfg_of_tle p1)))
@@ -3322,6 +3530,11 @@ Module Type LangRefine (IS1 : InterpreterStack) (IS2 : InterpreterStack) (AC1 : 
     L1_E1E2_orutt_strict
       (LLVM1.model_oom_L1 p1)
       (LLVM2.model_oom_L1 p2).
+
+  Definition model_E1E2_L2_orutt_strict p1 p2 :=
+    L2_E1E2_orutt_strict
+      (LLVM1.model_oom_L2 p1)
+      (LLVM2.model_oom_L2 p2).
 
   Import TranslateFacts.
   Import RecursionFacts.
@@ -9801,7 +10014,6 @@ Module Type LangRefine (IS1 : InterpreterStack) (IS2 : InterpreterStack) (AC1 : 
     }
   Qed.
 
-
   Lemma model_E1E2_01_orutt_strict :
     forall t1 t2 g1 g2,
       L0_E1E2_orutt_strict t1 t2 ->
@@ -9814,6 +10026,14 @@ Module Type LangRefine (IS1 : InterpreterStack) (IS2 : InterpreterStack) (AC1 : 
     apply E1E2_interp_intrinsics_orutt_strict; auto.
   Qed.
 
+  Lemma model_E1E2_12_orutt_strict :
+    forall t1 t2 ls1 ls2,
+      L1_E1E2_orutt_strict t1 t2 ->
+      local_stack_refine_strict ls1 ls2 ->
+      L2_E1E2_orutt_strict (interp_local_stack t1 ls1) (interp_local_stack t2 ls2).
+  Proof.
+  Admitted.
+
   Lemma model_E1E2_L1_orutt_strict_sound
     (p : list
            (LLVMAst.toplevel_entity
@@ -9824,6 +10044,19 @@ Module Type LangRefine (IS1 : InterpreterStack) (IS2 : InterpreterStack) (AC1 : 
     apply model_E1E2_01_orutt_strict;
       [ apply model_E1E2_L0_orutt_strict_sound
       | apply global_refine_strict_empty
+      ].
+  Qed.
+
+  Lemma model_E1E2_L2_orutt_strict_sound
+    (p : list
+           (LLVMAst.toplevel_entity
+              LLVMAst.typ
+              (LLVMAst.block LLVMAst.typ * list (LLVMAst.block LLVMAst.typ)))) :
+    model_E1E2_L2_orutt_strict p p.
+  Proof.
+    apply model_E1E2_12_orutt_strict;
+      [ apply model_E1E2_L1_orutt_strict_sound
+      | apply local_stack_refine_strict_empty
       ].
   Qed.
 
